\documentclass[10pt,a4paper]{article}
\usepackage[utf8]{inputenc}
\usepackage[ngerman]{babel}
\usepackage{amsmath}
\usepackage{amsfonts}
\usepackage{amssymb}
\usepackage{amsthm} % for proof-environment
\usepackage{bm} % for better \boldsymbol
\usepackage[left=2cm,right=2cm,top=2cm,bottom=2cm]{geometry}
\author{Leonard K\"onig}
\title{Beweis zu Aufgabe}
\date{2015-10-01}
%
\newtheorem*{beh}{Behauptung}
%
\begin{document}
\begin{beh}
\begin{align*}
x \wedge y \wedge z \equiv
& \left(x \rightarrow y \wedge z\right) \wedge \\
& \left(y \rightarrow x \wedge z\right) \wedge \\
& \left(z \rightarrow x \wedge y\right) \wedge \\
& \left(x \vee y \vee z \right)
\end{align*}
\end{beh}
%
%
\begin{proof}
\begin{align}
& \left(x \rightarrow y \wedge z\right) \wedge \notag\\
& \left(y \rightarrow x \wedge z\right) \wedge \notag\\
& \left(z \rightarrow x \wedge y\right) \wedge \notag\\
& \left(x \vee y \vee z \right) && \mid\text{ \glqq Verteilen\grqq\ vom \glq}\rightarrow\text{\grq}\\
\equiv
%
& \left(x \rightarrow y\right) \wedge \bm{\left(x \rightarrow z\right)} \wedge \notag\\
& \bm{\left(y \rightarrow x\right)} \wedge \left(y \rightarrow z\right) \wedge \notag\\
& \left(z \rightarrow x\right) \wedge  \bm{\left(z \rightarrow y\right)} \wedge \notag\\
& \left(x \vee y \vee z \right) && \mid\text{ Redundanzen tilgen}\\
\equiv
%
& \left(x  \bm{\rightarrow} y\right) \wedge
\left(y  \bm{\rightarrow} z\right) \wedge
\left(z  \bm{\rightarrow} x\right) \wedge \notag\\
& \left(x \vee y \vee z \right) && \mid\text{ \glq}\rightarrow\text{\grq\ ersetzen}\\
\equiv
%
& \left(\neg x \vee y\right) \wedge
\left(\neg y \vee z\right) \wedge
\left(\neg z \vee x\right) \wedge \notag\\
& \left(x \vee y \vee z\right) && \mid\text{ Distribuieren}\\
\equiv
%
%
& (\left(\neg x \vee y\right) \wedge \left(\neg y \vee z\right) \wedge  \bm{\left(\neg z \vee x\right)} \wedge \bm{x}) \vee \notag\\
& ( \bm{\left(\neg x \vee y\right)} \wedge \left(\neg y \vee z\right) \wedge \left(\neg z \vee x\right) \wedge  \bm{y}) \vee \notag\\
& (\left(\neg x \vee y\right) \wedge  \bm{\left(\neg y \vee z\right)} \wedge \left(\neg z \vee x\right) \wedge \bm{z}) && \mid\text{ Absorption}\\
\equiv
%
& ( \bm{\left(\neg x \vee y\right)} \wedge \left(\neg y \vee z\right) \wedge  \bm{x}) \vee \notag\\
& ( \bm{\left(\neg y \vee z\right)} \wedge \left(\neg z \vee x\right) \wedge  \bm{y}) \vee \notag\\
& (\left(\neg x \vee y\right) \wedge  \bm{\left(\neg z \vee x\right)} \wedge  \bm{z})
 && \mid\text{ Distribuieren}\\
\equiv
%
& [ (\bm{\left(\neg x \wedge x\right)} \vee \left(y \wedge x\right)) \wedge \left(\neg y \vee z\right)] \vee \notag\\
& [ (\bm{\left(\neg y \wedge y\right)} \vee \left(y \wedge z\right)) \wedge \left(\neg z \vee x\right)] \vee \notag\\
& [ (\bm{\left(\neg z \wedge z\right)} \vee \left(z \wedge x\right)) \wedge \left(\neg x \vee y\right)] && \mid\text{ Komplementarit\"at \& Neutralit\"at}\\
\equiv
%
& [\left(y \wedge x\right)) \wedge \left(\neg y \vee z\right)] \vee \notag\\
& [\left(y \wedge z\right)) \wedge \left(\neg z \vee x\right)] \vee \notag\\
& [\left(z \wedge x\right)) \wedge \left(\neg x \vee y\right)]
 && \mid\text{ Distribuieren}\\
\equiv
%
& [\left( \bm{\left(}y \wedge x \bm{\right)} \wedge \neg y) \vee ( \bm{\left(}y \wedge x \bm{\right)} \wedge z\right)] \vee \notag\\
& [\left( \bm{\left(}y \wedge z \bm{\right)} \wedge \neg z) \vee ( \bm{\left(}y \wedge z \bm{\right)} \wedge x\right)] \vee \notag\\
& [\left( \bm{\left(}z \wedge x \bm{\right)} \wedge \neg x) \vee ( \bm{\left(}z \wedge x \bm{\right)} \wedge y\right)]
 && \mid\text{ Assoziativit\"at}\\
\equiv
%
& [\left( \bm{y \wedge} x \wedge  \bm{\neg y}) \vee (y \wedge x \wedge z\right)] \vee \notag\\
& [\left(y \wedge  \bm{z \wedge \neg z}) \vee (y \wedge z \wedge x\right)] \vee \notag\\
& [\left(z \wedge  \bm{x \wedge \neg x}) \vee (z \wedge x \wedge y\right)]
 && \mid\text{ Komplementarit\"at \& Dominanz}\\
\equiv
%
& [\left(0) \vee (y \wedge x \wedge z\right)] \vee \notag\\
& [\left(0) \vee (y \wedge z \wedge x\right)] \vee \notag\\
& [\left(0) \vee (z \wedge x \wedge y\right)] && \mid\text{ Neutralit\"at}\\
\equiv
%
& \left(y \wedge x \wedge z\right) \vee
\left(y \wedge z \wedge x\right) \vee
\left(z \wedge x \wedge y\right) \vee && \mid\text{ Redundanz}\\
\equiv 
%
& z \wedge x \wedge y && \qedhere
\end{align}
\end{proof}
\pagenumbering{gobble}
\end{document}